add more view shift lemmata

IrisCore/BasicTypes.thy
@@ -8,6 +8,10 @@ subsubsection \<open>Disjoint set type\<close>
 text \<open> Set with extra bottom element to encode non-disjoint unions \<close>
 datatype 'a dset = DSet "'a set" | DBot
 
+fun dset_raw :: "'a dset \<Rightarrow> 'a set option" where
+  "dset_raw (DSet s) = Some s"
+| "dset_raw DBot = None"
+
 fun subdset_eq :: "'a dset \<Rightarrow> 'a dset \<Rightarrow> bool" (infix "\<subseteq>\<^sub>d" 50) where
   "subdset_eq (DSet s) (DSet t) = (s\<subseteq>t)"
 | "subdset_eq _ _ = False"
@@ -24,6 +28,21 @@ fun minus_dset :: "'a dset \<Rightarrow> 'a dset \<Rightarrow> 'a dset" where
 instance ..
 end
 
+lemma delem_dsubs: "i\<in>\<^sub>d d \<longleftrightarrow> DSet {i} \<subseteq>\<^sub>d d"
+  using dmember.elims(2) subdset_eq.elims(2) by fastforce
+
+lemma dsubs_dset: "d1 \<subseteq>\<^sub>d d2 \<Longrightarrow> \<exists>s1 s2. d1 = DSet s1 \<and> d2 = DSet s2"
+  using subdset_eq.elims(2) by fastforce
+
+lemma dsubs_raw: "d1 \<subseteq>\<^sub>d d2 \<Longrightarrow> \<exists>s1 s2. dset_raw d1 = Some s1 \<and> dset_raw d2 = Some s2"
+  using subdset_eq.elims(2) by fastforce
+
+lemma dminus_raw: "\<lbrakk>dset_raw d1 = Some s1\<rbrakk> \<Longrightarrow> \<exists>s3. dset_raw (d1 - d2) = Some s3"
+  by (metis dset.simps(3) dset_raw.elims minus_dset.simps(1) minus_dset.simps(2))
+
+lemma dsubs_minus_inter: "d1 \<subseteq>\<^sub>d d2 \<Longrightarrow> \<exists>s1 s3. Some s3 = (dset_raw (d2 - d1)) \<and> s1 \<inter> s3 = {}"
+  using dsubs_raw dminus_raw by (metis inf_bot_left)
+  
 subsubsection \<open>Disjoint finite set type\<close>
 text \<open> Finite set with extra bottom element to encode non-disjoint unions \<close>
 datatype 'a dfset = DFSet "'a fset" | DFBot
